separate min_max_disj and add disj_tre

theories/mut_excl.v
@@ -1,6 +1,6 @@
 From det Require Import prelude.
 From mathcomp Require Import all_ssreflect.
-From det Require Import tree tree_prop ctx tree_vars fresh unif.
+From det Require Import tree tree_prop ctx tree_vars fresh unif min_max_disj.
 
 Section good_mode.
   Definition arri t := if t is _ --i--> _ then true else false.
@@ -410,122 +410,6 @@ Proof.
   split => //.
   apply: (@fresh_tm_idempotent 0); rewrite//?(codomf0,idempotent_ren0,fdisjointX0,fsubsetUl)//.
   by rewrite/sum_mt domf0 codomf0 !fsetU0 !freshPU freshP1 H andbT; destruct n.
-Qed.
-
-Definition min_maxS (s:{fset V}) m M :=
-  forall x, IV x \in s -> m <= x < M.
-
-Lemma min_max_fresh_tm r m M q:
-  m <= M ->
-  min_maxS (codomf r) m M ->
-  let x := fresh_tm M r q in
-  min_maxS (codomf x.2) m x.1.
-Proof.
-  elim: q M r => /=[p|v|f Hf a Ha] M r// mm MM; last by (rewrite push; apply/Ha/Hf; rewrite//(leq_trans mm)//fresh_sub).
-  case: fndP => vr//=; rewrite codomf_setN//.
-  move=> x; rewrite 2!inE; case: eqP => [[->]|]; first by rewrite mm/=.
-  by move=> xm H; have /andP[->/leq_trans->]:= MM x H.
-Qed.
-
-Lemma min_max_fresh_atom r m M q:
-  m <= M ->
-  min_maxS (codomf r) m M ->
-  let x := fresh_atom M r q in
-  min_maxS (codomf x.1.2) m x.1.1.
-Proof. by case: q => //=t mm MM; rewrite !push/=; apply: min_max_fresh_tm. Qed.
-
-Lemma min_max_fresh_atoms r m M q:
-  m <= M ->
-  min_maxS (codomf r) m M ->
-  let x := fresh_atoms M r q in
-  min_maxS (codomf x.1.2) m x.1.1.
-Proof.
-  elim: q M r => //=[x xs IH] M r// mm MM; rewrite !push/=.
-  by apply/min_max_fresh_atom/IH/MM/mm/leq_trans/fresh_atoms_sub.
-Qed.
-
-Lemma min_maxP s:
-  min_maxS s 0 (fresh s).
-Proof.
-  move=> x xs; rewrite leq0n/=; case: (boolP (_ < _)) => //=.
-  by rewrite -leqNgt => /fresh_sub_notin; rewrite xs.
-Qed.
-
-Lemma min_max_fresh_tm0 fv q:
-  let x := fresh_tm fv fmap0 q in
-  min_maxS (codomf x.2) fv x.1.
-Proof.
-  move=> H/=.
-  have MM : min_maxS (codomf fmap0) fv fv by move=> x; rewrite /= codomf0.
-  by have := @min_max_fresh_tm fmap0 fv fv q (leqnn _) (MM _).
-Qed.
-
-Lemma min_maxU a b m M:
-  min_maxS a m M -> min_maxS b m M -> min_maxS (a `|` b) m M.
-Proof. by move=> M1 M2 x; rewrite inE => /orP[/M1|/M2]. Qed.
-
-Lemma min_max_fresh_rules fv r:
-  let x := fresh_rules fv r in
-  min_maxS (v_prog x.2) fv x.1.
-Proof.
-  elim: r fv => //=r rs IH m; rewrite !push/= v_prog_cons.
-  apply: min_maxU; last first.
-    move=> x H; have /andP[->/= Hx] := IH m x H.
-    by apply/leq_trans/fresh_rule_sub.
-  set X:= (fresh_rules _ _).1.
-  rewrite/fresh_rule; case: r => h b; rewrite /varsU_rhead/varsU_rprem !push/=.
-  set Y:= fresh_tm _ _ _.
-  apply: min_maxU .
-    have/= H:= @min_max_fresh_tm0 X h.
-    rewrite -/Y in H.
-    move=> x y.
-    have:= vars_tm_ren_sub (fresh_tm_sub1 X fmap0 h).
-    rewrite-/Y => Hx.
-    have /andP[Hl Hr] := H _ (fsubsetP Hx _ y).
-    apply/andP; split; last first.
-      by apply/leq_trans/fresh_atoms_sub.
-    apply/leq_trans/Hl/fresh_rules_sub.
-  elim: b => //-[|t]/= xs {}IH; rewrite !push/=vars_atoms_cons/=.
-    by rewrite fset0U.
-  apply: min_maxU; last first.
-    move=> x H.
-    have/andP[-> {}IH]/=:= IH x H.
-    apply: leq_trans IH _.
-    by apply/leq_trans/fresh_sub.
-  clear IH.
-  set F := fresh_atoms _ _ _.
-  set Z := fresh_tm _ _ _.
-  have xx: m <= F.1.1.
-    apply/leq_trans/fresh_atoms_sub/leq_trans/fresh_sub/fresh_rules_sub.
-  have yy: min_maxS (codomf F.1.2) m F.1.1.
-    have kk : m <= Y.1 by apply/leq_trans/fresh_sub/fresh_rules_sub.
-    have zz : min_maxS (codomf Y.2) m Y.1.
-      apply/min_max_fresh_tm; first by apply/fresh_rules_sub.
-      by rewrite codomf0//.
-    have/= H := @min_max_fresh_atoms Y.2 m Y.1 xs kk zz.
-    rewrite -/F in H.
-    by move=> x Hx; have /andP[->{}H] := H x Hx.
-  have/= H:= @min_max_fresh_tm F.1.2 m F.1.1 t xx yy.
-  rewrite-/Z/= in H.
-  move=> x y.
-  have:= vars_tm_ren_sub (fresh_tm_sub1 F.1.1 F.1.2 t).
-  rewrite-/Z => Hx.
-  by have/andP[->/=->] := H _ (fsubsetP Hx _ y).
-Qed.
-
-Lemma min_max_S_disj s1 s2 m1 m2 M1 M2:
-  M1 <= m2 ->
-  min_maxS s1 m1 M1 ->
-  min_maxS s2 m2 M2 ->
-  s1 # s2.
-Proof.
-  move=> mm H1 H2; apply/fdisjointP => -[x] xs1.
-  case: (boolP (_ \in _)) => //xs2.
-  have /andP[m1x xM1] := H1 _ xs1.
-  have /andP[m2x xM2] := H2 _ xs2.
-  have {xM1} xm2 := leq_trans xM1 mm.
-  have:= leq_trans xm2 m2x.
-  by rewrite ltnn.
 Qed.
 
 Lemma H_head_ren sP fv1 fv2 t xs fx fy q:
