theories/min_max_disj.v
@@ -1,0 +1,134 @@
+From det Require Import prelude.
+From mathcomp Require Import all_ssreflect.
+From det Require Import lang.
+From det Require Import tree tree_prop fresh.
+
+Definition min_maxS (s:{fset V}) m M :=
+  [forall x : s, let: IV x := val x in m <= x < M].
+
+Lemma min_max_fresh_tm r m M q:
+  m <= M ->
+  min_maxS (codomf r) m M ->
+  let x := fresh_tm M r q in
+  min_maxS (codomf x.2) m x.1.
+Proof.
+  elim: q M r => /=[p|v|f Hf a Ha] M r// mm MM; last by (rewrite push; apply/Ha/Hf; rewrite//(leq_trans mm)//fresh_sub).
+  case: fndP => vr//=; rewrite codomf_setN//.
+  apply/forallP => -[[x] xP]/=; move: xP.
+  rewrite 2!inE; case: eqP => [[->]|]; first by rewrite mm/=.
+  by move=> xm H; have /andP[->/leq_trans->]:= forallP MM [`H].
+Qed.
+
+Lemma min_max_fresh_atom r m M q:
+  m <= M ->
+  min_maxS (codomf r) m M ->
+  let x := fresh_atom M r q in
+  min_maxS (codomf x.1.2) m x.1.1.
+Proof. by case: q => //=t mm MM; rewrite !push/=; apply: min_max_fresh_tm. Qed.
+
+Lemma min_max_fresh_atoms r m M q:
+  m <= M ->
+  min_maxS (codomf r) m M ->
+  let x := fresh_atoms M r q in
+  min_maxS (codomf x.1.2) m x.1.1.
+Proof.
+  elim: q M r => //=[x xs IH] M r// mm MM; rewrite !push/=.
+  by apply/min_max_fresh_atom/IH/MM/mm/leq_trans/fresh_atoms_sub.
+Qed.
+
+Lemma min_maxP s:
+  min_maxS s 0 (fresh s).
+Proof.
+  apply/forallP => -[[x] xP]/=.
+  case: (boolP (_ < _)) => //=.
+  by rewrite -leqNgt => /fresh_sub_notin; rewrite xP.
+Qed.
+
+Lemma min_max_fresh_tm0 fv q:
+  let x := fresh_tm fv fmap0 q in
+  min_maxS (codomf x.2) fv x.1.
+Proof.
+  move=> /=.
+  have MM : min_maxS (codomf fmap0) fv fv.
+    by move=> t; apply/forallP => -[[x]]; rewrite /= codomf0//.
+  by have := @min_max_fresh_tm fmap0 fv fv q (leqnn _) (MM _).
+Qed.
+
+Lemma min_maxU a b m M:
+  min_maxS a m M -> min_maxS b m M -> min_maxS (a `|` b) m M.
+Proof. 
+  move=> M1 M2; apply/forallP => -[[x]xP]/=; move: xP; rewrite inE => /orP[]H.
+    by have:= forallP M1 [`H].
+  by have:= forallP M2 [`H].
+Qed.
+
+Lemma vars_tm_ren_codom_sub w t1: vars_tm t1 `<=` domf w -> vars_tm (ren w t1) `<=` codomf w.
+Proof.
+  elim: t1 => //=[v|f Hf a Ha].
+    by rewrite fsub1set => vw; rewrite in_fnd/=fsub1set in_codomf.
+  by rewrite !fsubUset => /andP[/Hf-> /Ha->].
+Qed.
+
+Lemma min_max_fresh_rules fv r:
+  let x := fresh_rules fv r in
+  min_maxS (v_prog x.2) fv x.1.
+Proof.
+  move=> /=; apply/forallP => -[[x]xP]/=.
+  elim: r fv xP => //=r rs IH fv; rewrite !push/= v_prog_cons.
+  rewrite 2!inE => /orP[]; last first.
+    move=> /IH/andP[->]/= Hx.
+    by apply/leq_trans/fresh_rule_sub.
+  set X:= (fresh_rules _ _).1.
+  rewrite/fresh_rule; case: r => h b; rewrite /varsU_rhead/varsU_rprem !push/=.
+  set Y:= fresh_tm _ _ _.
+  move=> /orP[].
+    have/= H:= @min_max_fresh_tm0 X h.
+    rewrite -/Y in H.
+    move=> H1.
+    have:= vars_tm_ren_codom_sub (fresh_tm_sub1 X fmap0 h).
+    rewrite-/Y => Hx.
+    have /andP[Hl Hr] := forallP H [`(fsubsetP Hx _ H1)].
+    apply/andP; split; last first.
+      by apply/leq_trans/fresh_atoms_sub.
+    apply/leq_trans/Hl/fresh_rules_sub.
+    Search fresh_atoms.
+  elim: b => //-[|t]/= xs {}IH; rewrite !push/=vars_atoms_cons/=.
+    by rewrite fset0U.
+  rewrite inE => /orP[]; last first.
+    move=> /IH/andP[->] H.
+    apply: leq_trans H _.
+    by apply fresh_sub.
+  clear IH.
+  set F := fresh_atoms _ _ _.
+  set Z := fresh_tm _ _ _.
+  have xx: fv <= F.1.1.
+    apply/leq_trans/fresh_atoms_sub/leq_trans/fresh_sub/fresh_rules_sub.
+  have yy: min_maxS (codomf F.1.2) fv F.1.1.
+    have kk : fv <= Y.1 by apply/leq_trans/fresh_sub/fresh_rules_sub.
+    have zz : min_maxS (codomf Y.2) fv Y.1.
+      apply/min_max_fresh_tm; first by apply/fresh_rules_sub.
+      by rewrite codomf0//; apply/forallP => -[].
+    have/= H := @min_max_fresh_atoms Y.2 fv Y.1 xs kk zz.
+    by rewrite -/F in H.
+  have/= H:= @min_max_fresh_tm F.1.2 fv F.1.1 t xx yy.
+  rewrite-/Z/= in H.
+  move=> Hx.
+  have:= vars_tm_ren_codom_sub (fresh_tm_sub1 F.1.1 F.1.2 t).
+  rewrite-/Z => Hy.
+  by have := forallP H [`(fsubsetP Hy _ Hx)].
+Qed.
+
+Lemma min_max_S_disj s1 s2 m1 m2 M1 M2:
+  M1 <= m2 ->
+  min_maxS s1 m1 M1 ->
+  min_maxS s2 m2 M2 ->
+  fdisjoint s1 s2.
+Proof.
+  move=> mm H1 H2; apply/fdisjointP => -[x] xs1.
+  case: (boolP (_ \in _)) => //xs2.
+  have /andP[m1x xM1] := forallP H1 [`xs1].
+  have /andP[m2x xM2] := forallP H2 [`xs2].
+  have {xM1} xm2 := leq_trans xM1 mm.
+  have:= leq_trans xm2 m2x.
+  by rewrite ltnn.
+Qed.
